New system for float literal notation, and float literal rewrites.
In float_lib.v, a new system for writing things like
  $"0.5f" $"1.73e-2"   etc., where what's in quotes is in C standard
  floating-point-literal notation, and $ is a tactic notation that
  eagerly converts this (as soon as Coq parses it) into a float or
  float32 constant value.  Useful in writing functional programs in Coq
  that contain floating-point constants.

Also in float_lib.v, a new system for creating rewrite rules to turn
Clight-abstract-syntax tree notation for floating-point constants
(which look like  `Float32.of_bits (Int.repr 1065353216)` for example)
into the Coq floating-point constant expression of your choice
(so long as it's actually equal, of course).  Useful in doing VST
refinement proofs about floating-point programs.

leapfrog_project/float_lib.v
@@ -26,6 +26,8 @@ Coercion float_of_Z: Z >-> float.
 
 Declare Scope F32.
 Delimit Scope F32 with F32.
+Declare Scope F64.
+Delimit Scope F64 with F64.
 
 Notation "x + y" := (Float32.add x y) (at level 50, left associativity) : F32.
 Notation "x - y"  := (Float32.sub x y) (at level 50, left associativity) : F32.
@@ -43,6 +45,23 @@ Notation "x <= y < z" := (x <= y /\ y < z)%F32 (at level 70, y at next level) : 
 Notation "x < y < z" := (x < y /\ y < z)%F32 (at level 70, y at next level) : F32.
 Notation "x < y <= z" := (x < y /\ y <= z)%F32 (at level 70, y at next level) : F32.
 
+Notation "x + y" := (Float.add x y) (at level 50, left associativity) : F64.
+Notation "x - y"  := (Float.sub x y) (at level 50, left associativity) : F64.
+Notation "x * y"  := (Float.mul x y) (at level 40, left associativity) : F64.
+Notation "x / y"  := (Float.div x y) (at level 40, left associativity) : F64.
+Notation "- x" := (Float.neg x) (at level 35, right associativity) : F64.
+
+Notation "x <= y" := (Float.cmp Cle x y = true) (at level 70, no associativity) : F64.
+Notation "x < y" := (Float.cmp Clt x y = true) (at level 70, no associativity) : F64.
+Notation "x >= y" := (Float.cmp Cge x y = true) (at level 70, no associativity) : F64.
+Notation "x > y" := (Float.cmp Cgt x y = true) (at level 70, no associativity) : F64.
+
+Notation "x <= y <= z" := (x <= y /\ y <= z)%F64 (at level 70, y at next level) : F64.
+Notation "x <= y < z" := (x <= y /\ y < z)%F64 (at level 70, y at next level) : F64.
+Notation "x < y < z" := (x < y /\ y < z)%F64 (at level 70, y at next level) : F64.
+Notation "x < y <= z" := (x < y /\ y <= z)%F64 (at level 70, y at next level) : F64.
+
+
 Ltac eq_hnf := 
  lazymatch goal with |- ?A = ?B =>
    let x := fresh "x" in
@@ -50,6 +69,8 @@ Ltac eq_hnf :=
     set (x:=B); hnf in x; subst x
  end.
  
+Definition f_lit (s: string) {T: Type} {x: T} := x.
+
 Ltac prove_float_constants_equal :=
  lazymatch goal with
  | |- @eq ?t ?A ?B =>
@@ -109,6 +130,277 @@ Proof.
 (* Almost certainly true, but a royal pain to prove. *)
 Abort.
 
+
+(* BEGIN system for parsing and rewriting floating-point literals.
+
+  FEATURE 1: literals expressed on C notation.
+  How to use it: In notation scope F32 or F64, the term  ($ s) 
+  produces a fully reduced floating-point value of type float32 or float,
+  where the string s is a floating-point literal in C standard notation.
+  Examples: $"0.5f", $".5f", $"5E-1f" all produce the float32 value 1/2;
+      $"0.5", $".5", $"5E-1" all produce the 64-bit float value 1/2.
+  Important:  No matter whether you're in Notation Scope F32 or F64,
+  $"0.5" is a 64-bit floating point constant whose type is [float], and
+  $"0.5f" is a 32-bit floating point constant of type [float32].
+
+  FEATURE 2: Clight abstract syntax trees contain a lot of 
+  constants of the form, (Float32.of_bits (Int.repr 1065353216)).
+  You might want to rewrite that into something like 
+  (float_of_Z 1)  $"1.0f"  or   one     (assuming that "one" is your own
+   Definition that unfolds to a floating-point constant).
+ To do that, you can write any of these:
+
+   Hint Rewrite float_const_rewrite "1.0f" : float_const.
+   Hint Rewrite float_const_rewrite (float_of_Z 1) : float_const.
+   Hint Rewrite float_const_rewrite one : float_const.
+
+   float_const_rewrite is a tactic that takes an argument of type 
+   string, or of type float32 or float.   It computes that argument [s]
+   into a floating point constant, calculates an integer constant [n], 
+   and produces the proof of an equation,
+    Float32.of_bits (Int.repr n) = s
+  which you can then use as a rule in a Hint Rewrite database.
+  (or Float.bits, as appropriate, if s is a 64-bit float).
+
+   It's a good idea to pick only one of the above, because otherwise
+   you'll get 3 different rewrite rules all with the same l.h.s,
+   which is not so useful.
+
+*)
+
+Definition Bparse_float32 := Bparse 24 128 (eq_refl _) (eq_refl _) 10.
+Definition Bparse_float := Bparse 53 1024 (eq_refl _) (eq_refl _) 10.
+
+Fixpoint parse_decimal (b: N) (len: N) (s: string) : N * N * string :=
+ match s with
+ | EmptyString => (b,len,s)
+ | String c r => let c' := Ascii.N_of_ascii c in
+             if andb (N.leb 48 c') (N.ltb c' 58) 
+             then parse_decimal (b*10+c'-48)%N  (len+1) r
+             else (b,len,s)
+ end.
+ 
+Import Ascii.
+Import ListNotations.
+Require compcert.common.Errors.
+
+Inductive float_type := ft_single | ft_double.
+
+Definition parse_float_exponent'  (sign:bool) (mantissa: N) (len2: N) (esign: Z) (e len3: N) (ft: float_type) : 
+             Errors.res (bool * option (positive*Z) * float_type) :=
+          if N.eqb len3 0 
+                     then Errors.Error [Errors.MSG "No digits in exponent"]
+                   else if N.eqb mantissa 0 then Errors.OK(sign,None,ft)
+                   else Errors.OK(sign,Some(Pos.pred (N.succ_pos mantissa),
+                                          esign * Z.of_N e - Z.of_N len2), ft).
+
+Definition parse_float_exponent (sign:bool) (mantissa: N) (len1 len2: N) (esign: Z) (s: string) : 
+             Errors.res (bool * option (positive*Z) * float_type) :=
+  if N.eqb (len1+len2) 0
+  then Errors.Error [Errors.MSG "No digits before or after decimal point"]
+  else match parse_decimal 0 0 s with
+          | (_,0%N, _) => Errors.Error [Errors.MSG "Missing exponent"]
+          | (e,len3,EmptyString) => parse_float_exponent' sign mantissa len2 esign e len3 ft_double
+          | (e,len3,String ("f"|"F") EmptyString) => parse_float_exponent' sign mantissa len2 esign e len3 ft_single
+          | (e,len3,String ("f"|"F") _) => Errors.Error [Errors.MSG "Junk after f suffix"]
+          | (_,_, String _ _) => Errors.Error [Errors.MSG "Junk after exponent"]
+          end.
+
+Definition parse_float_noexponent (sign:bool) (mantissa: N) (len1 len2: N) (ft: float_type) : 
+             Errors.res (bool * option (positive*Z) * float_type) :=
+     if N.eqb mantissa 0
+        then if N.eqb (len1+len2) 0
+                       then Errors.Error [Errors.MSG "No digits before or after decimal point"]
+                       else Errors.OK (sign,None,ft)
+                    else Errors.OK (sign, Some
+                                  (Pos.pred (N.succ_pos mantissa),
+                                  (- Z.of_N len2)), ft).
+
+Definition parse_float_mantissa2 (sign: bool) (mantissa: N) (len1 len2: N) (s: string) : 
+             Errors.res (bool * option (positive*Z) * float_type) :=
+ match s with
+ | String ("e"|"E") (String "+" r) => parse_float_exponent sign mantissa len1 len2 1 r
+ | String ("e"|"E") (String "-" r) => parse_float_exponent sign mantissa len1 len2 (-1) r
+ | String ("e"|"E") r => parse_float_exponent sign mantissa len1 len2 1 r
+ | EmptyString => parse_float_noexponent sign mantissa len1 len2 ft_double
+ | String ("f"|"F") EmptyString => parse_float_noexponent sign mantissa len1 len2 ft_single
+ | _ => Errors.Error [Errors.MSG "Cannot parse the rest of this float:"; Errors.MSG s]
+ end.
+
+Definition parse_float_mantissa1 (sign: bool) (s: string) :
+             Errors.res (bool * option (positive*Z) * float_type) :=
+ let '(i,len1,s1) := parse_decimal 0%N 0 s in
+ match s1 with 
+ | String "." r => let '(j,len2,s2) := parse_decimal i 0 r in
+                          parse_float_mantissa2 sign j len1 len2 s2
+ | _ => parse_float_mantissa2 sign i len1 0 s1
+ end.
+
+Definition parse_float (s: string) :=
+ match s with
+ | String "+" r => parse_float_mantissa1 true r
+ | String "-" r => parse_float_mantissa1 false r
+ | _ => parse_float_mantissa1 true s
+ end.
+
+Ltac f_lit_exact s x := let y := eval simpl in x in exact (@f_lit s _ y).
+
+Ltac f_lit_aux cont s :=
+ let r := constr:(parse_float s) in
+ let r := eval vm_compute in r in
+ lazymatch r with
+ | Errors.Error ?c => fail 0 c
+ | Errors.OK (?p, None,ft_single) => 
+  lazymatch p with
+  | true => cont s constr:(Float32.zero)
+  | false =>cont s constr:(Float32.neg Float32.zero)
+ end
+ | Errors.OK (?p, None,ft_double) => 
+  lazymatch p with
+  | true => cont s constr:(Float.zero)
+  | false =>cont s constr:(Float.neg Float.zero)
+ end
+ | Errors.OK (?p, Some (?m,?e),ft_single) =>
+   let x := constr:(Bparse_float32 m e) in
+   let x := eval hnf in x in 
+   let x := eval simpl in x in 
+  lazymatch p with
+  | true => cont s x
+  | false =>cont s (Float32.neg x)
+ end 
+ | Errors.OK (?p, Some (?m,?e),ft_double) =>
+   let x := constr:(Bparse_float m e) in
+   let x := eval hnf in x in 
+   let x := eval simpl in x in 
+  lazymatch p with
+  | true => cont s x
+  | false =>cont s (Float.neg x)
+ end 
+end.
+
+Ltac f_lit s := f_lit_aux f_lit_exact s.
+
+Lemma constant_rewrite32 (x: float32):
+  forall n, n = Bits.bits_of_b32 x ->
+  Float32.of_bits (Int.repr n) = x.
+Proof.
+ intros. subst.
+ cbv delta [Float32.of_bits]; cbv beta.
+ rewrite Int.unsigned_repr.
+ unfold Bits.b32_of_bits.
+ unfold Bits.bits_of_b32.
+ rewrite Bits.binary_float_of_bits_of_binary_float.
+ auto.
+ unfold Bits.bits_of_b32.
+ assert (Int.max_unsigned + 1 = Int.modulus) by reflexivity.
+ assert (0 <= Bits.bits_of_binary_float 23 8 x < Int.modulus); [ | lia].
+ clear H.
+ apply Bits.bits_of_binary_float_range; reflexivity.
+Qed.
+
+Lemma constant_rewrite64 (x: float):
+  forall n, n = Bits.bits_of_b64 x ->
+  Float.of_bits (Int64.repr n) = x.
+Proof.
+ intros. subst.
+ cbv delta [Float.of_bits]; cbv beta.
+ rewrite Int64.unsigned_repr.
+ unfold Bits.b64_of_bits.
+ unfold Bits.bits_of_b64.
+ rewrite Bits.binary_float_of_bits_of_binary_float.
+ auto.
+ unfold Bits.bits_of_b64.
+ assert (Int64.max_unsigned + 1 = Int64.modulus) by reflexivity.
+ assert (0 <= Bits.bits_of_binary_float 52 11 x < Int64.modulus); [ | lia].
+ clear H.
+ apply Bits.bits_of_binary_float_range; reflexivity.
+Qed.
+
+Ltac compute_Float_bits f h :=
+ let h := eval hnf in h in 
+ let h' := eval cbv [Float32.zero Float32.div Float32.mul Float32.add Float32.sub Float32.neg
+                             Float.zero Float.div Float.mul Float.add Float.sub Float.neg]
+                              in h in
+  let n := constr:(f h') in
+           let n' := eval compute in n in constr:(n').
+
+Ltac float_const h :=
+ match type of h with
+ | string => 
+          f_lit_aux f_lit_x h
+ | ?t =>
+ tryif unify t float32 
+ then let n := compute_Float_bits Bits.bits_of_b32 h in
+     exact (constant_rewrite32 h n (eq_refl _))
+ else  tryif unify t float 
+ then let n := compute_Float_bits Bits.bits_of_b64 h in
+          exact (constant_rewrite64 h n (eq_refl _))
+ else fail 0  "This expression does not have type float or float32:" h
+ end
+with f_lit_x s x :=
+  let y := eval simpl in x in float_const (@f_lit s _ y).
+
+
+
+Module FloatLiteralNotation.
+ Notation "$ s" := (ltac:(f_lit s%string)) (at level 1, only parsing) : F32.
+ Notation "$ s" := (ltac:(f_lit s%string)) (at level 1, only parsing) : F64.
+ Notation "'float_const_rewrite' s" := (ltac:(float_const s%string)) (at level 1, only parsing).
+End FloatLiteralNotation.
+
+Import FloatLiteralNotation.
+
+Local Open Scope F32.
+
+(* Unit tests *)
+
+Goal $"0f" =  Float32.zero.
+prove_float_constants_equal. Abort.
+Goal $"0e6f"  =  Float32.zero.
+prove_float_constants_equal. Abort.
+Goal $"-0.5f"  =  Float32.neg (Float32.div 1 2).
+prove_float_constants_equal. Abort.
+Goal $".5f"  =  Float32.div 1 2.
+prove_float_constants_equal. Abort.
+Goal $".05E1f"  =  Float32.div 1 2.
+prove_float_constants_equal. Abort.
+Goal $".05E+1f"  =  Float32.div 1 2.
+prove_float_constants_equal. Abort.
+Goal $".05E+1"  =  Float.div 1 2.
+prove_float_constants_equal. Abort.
+Goal $"5E-1"  =  Float.div 1 2.
+prove_float_constants_equal. Abort.
+Goal $"1.5F"  =  (Float32.div 3 2).
+prove_float_constants_equal. Abort.
+
+Ltac test_flit_error s e :=
+ let r := constr:(parse_float s) in
+ let r := eval compute in r in
+ lazymatch r with
+ | Errors.Error ?c => 
+   tryif unify c (map Errors.MSG e) then exact True else fail 0 c
+ end.
+
+Local Open Scope string.
+Goal ltac:(test_flit_error "." ["No digits before or after decimal point"]). Abort.
+Goal ltac:(test_flit_error "3g." ["Cannot parse the rest of this float:";"g."]). Abort.
+
+Goal False.
+assert (H := float_const_rewrite "0").
+match type of H with Float.of_bits (Int64.repr 0) = f_lit "0" => idtac end.
+Abort.
+
+Goal False.
+assert (H := float_const_rewrite (float_of_Z 1)).
+match type of H with Float.of_bits (Int64.repr _) = float_of_Z 1 => idtac end.
+Abort.
+
+Goal False.
+assert (H := float_const_rewrite (float32_of_Z 1)).
+match type of H with Float32.of_bits (Int.repr _) = float32_of_Z 1 => idtac end.
+Abort.
+
+(* END system for parsing floating-point literals *)
 
 
 
